concurrency/machine_semantics.v
@@ -41,7 +41,7 @@ Record ConcurSemantics {G TID SCH TR C M: Type} : Type :=
     ; conc_halted : SCH -> C -> option val
     ; thread_step : G -> SCH -> C -> M -> C -> M -> Prop 
     ; machine_step : G -> SCH -> TR -> C -> M -> SCH -> TR -> C -> M -> Prop 
-    ; runing_thread : C -> option TID
+    ; runing_thread : C -> TID -> Prop
     ; thread_step_not_halted: 
       forall ge  U m q  m' q', thread_step ge U q m q' m' -> conc_halted U q = None
     ; machine_step_not_halted: 
